common/Memtype.v
@@ -1872,7 +1872,6 @@ for [unchanged_on]. *)
       (FAP2: frame_at_pos (stack_adt m2) O f2)
       (FI: tframe_inject j (perm m1) (f1::nil) f2)
       (HP: has_perm_frame (perm m1) j f1)
-      (SZ2: Forall (fun f => Forall (fun f =>0 = frame_adt_size f) f)%Z (stack_adt m2)) 
       (RSB: record_stack_blocks m1 f1 = Some m1')
       (G0: g O = Some O),
       inject j g m1' m2;
@@ -1881,7 +1880,7 @@ for [unchanged_on]. *)
     forall (m1 m1' m2 : mem) (j : meminj) g,
       inject j g m1 m2 ->
       unrecord_stack_block m1 = Some m1' ->
-      (forall i j, g i = Some j -> j = O) ->
+      (* (forall i j, g i = Some j -> j = O) -> *)
       (forall b, is_stack_top (stack_adt m1) b -> forall o k p, ~ perm m1 b o k p) ->
       g 1%nat = Some O ->
       (* size_stack (stack_adt m2) <= size_stack (stack_adt m1') -> *)
